compiler1/pat_to_closScript.sml
@@ -150,7 +150,7 @@ val compile_def = tDefine"compile"`
     Let [Op (SetGlobal n) (REVERSE (MAP compile es))]
       (Op (Cons (tuple_tag+pat_tag_shift)) [])) ∧
   (compile (App (Tag_eq n l) es) =
-    Op (TagEq (n+pat_tag_shift) l) (REVERSE (MAP compile es))) ∧
+    Op (TagLenEq (n+pat_tag_shift) l) (REVERSE (MAP compile es))) ∧
   (compile (App (El n) es) =
     Let (REVERSE (MAP compile es))
       (Op El [Op (Const &n) []; Var 0])) ∧
